ETCSList.sml
@@ -1,0 +1,37 @@
+(*
+collect the set of all sets of of sets of (n,a) pairs such that 
+{} in the set 
+if l is in in the set, then for every a\in A, l ∪ (CARD l,a) is in the set
+
+*)
+
+ 
+val Lists_cond_ex = prove_store("Lists_cond_ex",
+e0
+(rpt strip_tac >> 
+ qby_tac
+ ‘?P0. !ls. P0 o ls = TRUE <=> IN(Empty(N * A),ls)’ >--
+ (qexists_tac ‘Mem(Exp(N * A, 1 + 1)) o 
+             Pa(Empty(N * A) o To1(Exp(Exp(N * A, 1 + 1), 1 + 1)),id(Exp(Exp(N * A, 1 + 1), 1 + 1)))’
+ >> rw[o_assoc,Pa_distr,IN_def] >>
+ once_rw[one_to_one_id] >> rw[idL,idR,True1TRUE]) >>
+ pop_assum strip_assume_tac >>
+ qby_tac
+ ‘?P1. !a:1->A l ls.
+    P1 o Pa(a,Pa(l,ls)) = TRUE<=>
+    !n. hasCard(ls,n) ==> 
+ !a. IN(Ins(Pa(n,a),l), ls)’ >-- 
+(qexists_tac
+ ‘Mem(Exp(N * A, 1 + 1)) o 
+  Pa(Ins(
+     Pa
+     (CARD
+      (p32(A,Exp(N * A, 1 + 1),Exp(Exp(N * A, 1 + 1),1+1))), 
+      p31(A,Exp(N * A, 1 + 1),Exp(Exp(N * A, 1 + 1),1+1))),
+     p32(A,Exp(N * A, 1 + 1),Exp(Exp(N * A, 1 + 1),1+1))),
+)
+(form_goal “!A.?P. !ls.P o ls = TRUE <=>
+IN(Empty(N * A),ls) &
+ !l. IN(l,ls) ==>
+ !n. hasCard(ls,n) ==> 
+ !a. IN(Ins(Pa(n,a),l), ls)”)
